Switch to finite maps from std++

src/Containers.v
@@ -1,130 +1,176 @@
 From Coq Require Import ProofIrrelevance.
-From Containers Require Export OrderedType.
-From Containers Require OrderedTypeEx.
-From Containers Require SetListInstance.
-From Containers Require MapListInstance.
-From Containers Require MapFacts.
-From Containers Require SetProperties.
+From Coq Require Import ZArith.
+From stdpp Require Import gmap.
 From Coq Require Import List.
+From SmartContracts Require Import Monads.
 Import ListNotations.
 
-Notation FSet := SetInterface.set.
-
-Module FSet.
-  Notation empty := SetInterface.empty.
-  Notation add := SetInterface.add.
-  Notation mem := SetInterface.mem.
-  Notation remove := SetInterface.remove.
-  Notation elements := SetInterface.elements.
-  Notation size := SetInterface.cardinal.
-  Notation of_list := SetProperties.of_list.
-
-  (* TODO: We should really use setoids instead of this hacky crap... *)
-  Proposition of_elements_eq
-              {A : Type}
-              {a_order : OrderedType A}
-              (s : FSet A)
-              : of_list (elements s) = s.
-  Proof.
-    destruct s as [l l_sorted].
-    unfold SetProperties.of_list.
-    Transparent SetInterface.empty.
-    Transparent SetInterface.elements.
-    unfold SetInterface.empty.
-    unfold SetListInstance.SetList_FSet.
-    unfold SetList.empty.
-    unfold SetList.S.empty.
-    simpl.
-    induction l as [| hd tl IHl].
-    - simpl.
-      assert (SetList.S.empty_sort a_order = l_sorted) by apply proof_irrelevance.
-      subst; reflexivity.
-    - assert (decomposable: forall s1 s2 : SetList.set A, SetList.this s1 = SetList.this s2 -> s1 = s2).
-      + intros [l1 l1_sorted] [l2 l2_sorted].
-        simpl.
-        intros l1_eq_l2.
-        subst.
-        replace l2_sorted with l1_sorted by apply proof_irrelevance.
-        reflexivity.
-      + apply decomposable.
-        inversion l_sorted as [| a b tl_sorted hd_sorted]; subst.
-        simpl in *.
-        rewrite IHl with (l_sorted := tl_sorted).
-        Transparent SetInterface.add.
-        unfold SetInterface.add.
-        unfold SetList.add.
-        simpl.
-        unfold SetList.S.add.
-        destruct tl as [| hd' tl_tl].
-        * reflexivity.
-        * inversion hd_sorted as [|? ? hd_hd'_lt]; subst.
-          destruct (OrderedType.compare_dec hd hd').
-          -- reflexivity.
-          -- order.
-          -- order.
-  Qed.
-End FSet.
-
-Notation FMap := MapInterface.dict.
+Notation FMap := gmap.gmap.
 
 Module FMap.
-  Notation empty := MapInterface.empty.
-  Arguments empty {_ _ _ _}.
-  Notation add := MapInterface.add.
-  Notation find := MapInterface.find.
-  Notation mem := MapInterface.mem.
-  Notation remove := MapInterface.remove.
-  Notation elements := MapInterface.elements.
-  Notation size := MapInterface.cardinal.
-  Notation of_list := MapFacts.of_list.
+  Generalizable All Variables.
+  Notation empty := stdpp.base.empty.
+  Notation add := stdpp.base.insert.
+  Notation find := stdpp.base.lookup.
+  Definition mem `{base.Lookup K V M} (i : K) (m : M) :=
+    match base.lookup i m with
+    | Some _ => true
+    | None => false
+    end.
+
+  Notation remove := stdpp.base.delete.
+  Notation elements := fin_maps.map_to_list.
+  Notation size := stdpp.base.size.
+  Notation of_list := fin_maps.list_to_map.
 
   Proposition of_elements_eq
               {A B : Type}
-              {_ : OrderedType A}
+              `{countable.Countable A}
               (m : FMap A B)
               : of_list (elements m) = m.
   Proof.
-    destruct m as [l l_sorted].
-    unfold MapList.M.dict in *.
-    unfold MapFacts.of_list.
-    Transparent MapInterface.empty.
-    Transparent MapInterface.elements.
-    unfold MapInterface.empty.
-    unfold MapListInstance.MapList_FMap.
-    unfold MapList.empty.
-    unfold MapList.M.empty.
-    simpl.
-    induction l as [| hd tl IHl].
-    - simpl.
-      assert (MapList.M.empty_sorted B = l_sorted) by apply proof_irrelevance.
-      subst; reflexivity.
-    - assert (decomposable: forall m1 m2 : MapList.dict A B, MapList.this m1 = MapList.this m2 -> m1 = m2).
-      + intros [l1 l1_sorted] [l2 l2_sorted].
-        simpl.
-        intros l1_eq_l2.
-        subst.
-        replace l2_sorted with l1_sorted by apply proof_irrelevance.
-        reflexivity.
-      + apply decomposable.
-        simpl.
-        inversion l_sorted as [| a b tl_sorted hd_sorted].
-        subst.
-        rewrite IHl with (l_sorted := tl_sorted).
-        Transparent MapInterface.add.
-        unfold MapInterface.add.
-        unfold MapList.add.
-        simpl.
-        unfold MapList.M.add.
-        destruct hd as [k v].
-        simpl.
-        destruct tl as [| [k' v'] tl_tl].
-        * reflexivity.
-        * inversion hd_sorted as [|? ? k_k'_lt]; subst.
-          unfold MapList.M.K.ltk in k_k'_lt.
-          simpl in *.
-          destruct (compare_dec k k').
-          -- reflexivity.
-          -- order.
-          -- order.
+    apply fin_maps.list_to_map_to_list.
   Qed.
 End FMap.
+
+Instance empty_set_eq_dec : stdpp.base.EqDecision Empty_set.
+Proof. decidable.solve_decision. Defined.
+Program Instance empty_set_countable : countable.Countable Empty_set :=
+  {| countable.encode e := 1%positive; countable.decode d := None; |}.
+Solve Obligations with contradiction.
+
+(* The default list countable instance is exponential. For instance,
+   1000%positive takes around 10 bits to describe, but
+   countable.encode [1000%positive] returns a positive taking around
+   1000 bits to describe. This is because it writes everything out
+   in unary. Here is a more efficient implementation that works by
+   duplicating the bits of each element and separating them by
+   1~0. *)
+Remove Hints countable.list_countable : typeclass_instances.
+Section ListCountable.
+  Context `{countable.Countable A}.
+  Open Scope positive.
+
+  Fixpoint encode_single (p acc : positive) : positive :=
+    match p with
+    | 1 => acc
+    | p'~0 => encode_single p' (acc~0~0)
+    | p'~1 => encode_single p' (acc~1~1)
+    end.
+
+  Fixpoint encode_list' (l : list A) (acc : positive) : positive :=
+    match l with
+    | [] => acc
+    | hd :: tl => encode_list' tl (encode_single (encode hd) (acc~1~0))
+    end.
+
+  Definition encode_list l := encode_list' l 1.
+
+  Fixpoint decode_list'
+           (p : positive)
+           (acc_l : list A)
+           (acc_elm : positive)
+    : option (list A) :=
+      match p with
+      | 1 => Some acc_l
+      | p'~0~0 => decode_list' p' acc_l (acc_elm~0)
+      | p'~1~1 => decode_list' p' acc_l (acc_elm~1)
+      | p'~1~0 => do elm <- countable.decode acc_elm;
+                  decode_list' p' (elm :: acc_l) 1
+      | _ => None
+      end.
+
+  Definition decode_list (p : positive) : option (list A) :=
+    decode_list' p [] 1.
+
+  Lemma encode_single_app (p acc : positive) :
+    encode_single p acc = acc ++ encode_single p 1.
+  Proof.
+    generalize dependent acc.
+    induction p.
+    - intros acc.
+      simpl.
+      rewrite IHp.
+      rewrite (IHp 7).
+      rewrite Papp_assoc.
+      reflexivity.
+    - intros acc.
+      simpl.
+      rewrite IHp.
+      rewrite (IHp 4).
+      rewrite Papp_assoc.
+      reflexivity.
+    - intros acc.
+      reflexivity.
+  Qed.
+
+  Lemma encode_list'_app (l : list A) (acc : positive) :
+    encode_list' l acc = acc ++ encode_list' l 1.
+  Proof.
+    generalize dependent acc.
+    induction l as [| hd tl IHl].
+    - intros acc; reflexivity.
+    - intros acc.
+      simpl.
+      rewrite IHl.
+      rewrite (IHl (encode_single _ _)).
+      rewrite Papp_assoc.
+      rewrite (encode_single_app _ 6).
+      rewrite Papp_assoc.
+      simpl.
+      rewrite <- encode_single_app.
+      reflexivity.
+  Qed.
+
+  Lemma decode_list'_single (p prefix : positive) (l : list A) :
+    decode_list' (prefix ++ encode_single p 1) l 1 = decode_list' prefix l p.
+  Proof.
+    generalize dependent prefix.
+    induction p.
+    - intros.
+      simpl.
+      rewrite encode_single_app.
+      rewrite Papp_assoc.
+      rewrite IHp.
+      reflexivity.
+    - intros.
+      simpl.
+      rewrite encode_single_app.
+      rewrite Papp_assoc.
+      rewrite IHp.
+      reflexivity.
+    - reflexivity.
+  Qed.
+
+  Lemma decode_list'_list (prefix : positive) (l acc : list A) :
+    decode_list' (prefix ++ encode_list' l 1) acc 1 = decode_list' prefix (l ++ acc) 1.
+  Proof.
+    generalize dependent prefix.
+    generalize dependent acc.
+    induction l as [| hd tl IHl].
+    - reflexivity.
+    - intros acc prefix.
+      simpl.
+      rewrite encode_list'_app.
+      rewrite Papp_assoc.
+      rewrite IHl.
+      rewrite encode_single_app.
+      rewrite Papp_assoc.
+      rewrite decode_list'_single.
+      simpl.
+      rewrite decode_encode.
+      reflexivity.
+  Qed.
+
+  Global Program Instance list_countable : countable.Countable (list A) :=
+    {| encode := encode_list; decode := decode_list; |}.
+  Next Obligation.
+    intros l.
+    unfold encode_list, decode_list.
+    replace (encode_list' _ _) with (1 ++ encode_list' l 1) by apply Papp_1_l.
+    rewrite decode_list'_list.
+    simpl.
+    rewrite app_nil_r.
+    reflexivity.
+  Qed.
+End ListCountable.
